coq/Langs/S.v
@@ -162,7 +162,7 @@ Inductive expr : Type :=
 | Xabort : expr
 .
 Coercion Xres : ferr >-> expr.
-#[local]
+#[global]
 Instance expr__Instance : ExprClass expr := {}.
 
 (** Checks wether a given expression contains a delete of the given var *)
@@ -289,7 +289,7 @@ Inductive evalctx : Type :=
 | Kreturn (K : evalctx) : evalctx
 | Kcall (foo : vart) (K : evalctx) : evalctx
 .
-#[local]
+#[global]
 Instance evalctx__Instance : EvalCtxClass evalctx := {}.
 Inductive ety : Type :=
 | Tarrow : ty -> ty -> ety
@@ -1281,7 +1281,7 @@ Definition eventeq (e1 e2 : event) : bool :=
   | _, _ => false
   end
 .
-#[local]
+#[global]
 Instance Event__Instance : TraceEvent event := {}.
 (** Pretty-printing function for better debuggability *)
 Definition string_of_event (e : event) :=
@@ -1308,7 +1308,7 @@ Definition string_of_event (e : event) :=
 
 (** A runtime program is a state plus an expression. *)
 Definition rtexpr : Type := (option state) * expr.
-#[local]
+#[global]
 Instance rtexpr__Instance : RuntimeExprClass rtexpr := {}.
 (* '▷' is `\triangleright and '↯' is `\lightning`` *)
 Notation "Ω '▷' e" := ((((Some (Ω)) : option state), (e : expr)) : rtexpr) (at level 81).
@@ -1382,9 +1382,9 @@ Inductive pstep : PrimStep :=
     Some H' = Hgrow H n ->
     (F ; Ξ ; ξ ; H ; Δ) ▷ Xnew x n e --[ (Salloc (addr ℓ) n) ]--> (F'' ; Ξ ; ξ ; H' ; Δ') ▷ (subst x e (Fvar z))
 .
-#[local]
+#[global]
 Existing Instance pstep.
-#[local]
+#[global]
 Hint Constructors pstep : core.
 
 Lemma pstep_is_nodupinv_invariant Ω e Ω' e' a :
@@ -1701,7 +1701,7 @@ Lemma pstep_compat_weaken e :
   Some e = pstep_compatible e ->
   Some e = pestep_compatible e.
 Proof. induction e; now cbn. Qed.
-#[local]
+#[global]
 Hint Resolve pstep_compat_weaken call_pestep_compat return_pestep_compat : core.
 
 (** Environment Semantics extended with context switches *)
@@ -1727,9 +1727,9 @@ Inductive estep : CtxStep :=
     Ω ▷ e --[ Scrash ]--> ↯ ▷ stuck ->
     Ω ▷ e0 ==[ Scrash ]==> ↯ ▷ stuck
 .
-#[local]
+#[global]
 Existing Instance estep.
-#[local]
+#[global]
 Hint Constructors estep : core.
 
 Lemma estep_is_nodupinv_invariant Ω e Ω' e' a :
